backends/lean/Aeneas/Tactic/Step/Tests/HigherOrder.lean
@@ -17,8 +17,8 @@ theorem applyF_spec (f : U32 → Result U32) (x : U32)
 /--
 info: Try this:
 
-  [apply]     let* ⟨ y, y_post ⟩ ← [ +inferPost ] applyF_spec
-    case hf => let* ⟨ ⟩ ← [ +inferPost ] U32.add_spec
+  [apply]     let* ⟨ y, y_post ⟩ ← [ +inferPost ] applyF_spec_step
+    case hf => let* ⟨ ⟩ ← [ +inferPost ] U32.add_spec_step
     agrind
 -/
 #guard_msgs in
@@ -43,9 +43,9 @@ theorem callPair_spec (f g : U32 → Result U32) (xy : U32 × U32)
 /--
 info: Try this:
 
-  [apply]     let* ⟨ ab, ab_post1, ab_post2 ⟩ ← [ +inferPost ] callPair_spec
-    case hf => let* ⟨ ⟩ ← [ +inferPost ] U32.add_spec
-    case hg => let* ⟨ ⟩ ← [ +inferPost ] U32.add_spec
+  [apply]     let* ⟨ ab, ab_post1, ab_post2 ⟩ ← [ +inferPost ] callPair_spec_step
+    case hf => let* ⟨ ⟩ ← [ +inferPost ] U32.add_spec_step
+    case hg => let* ⟨ ⟩ ← [ +inferPost ] U32.add_spec_step
     agrind
 -/
 #guard_msgs in
@@ -70,11 +70,11 @@ theorem callFThenG_spec (f g : U32 → Result U32) (x : U32)
 /--
 info: Try this:
 
-  [apply]     let* ⟨ y, y_post ⟩ ← [ +inferPost ] callFThenG_spec
-    case hf => let* ⟨ ⟩ ← [ +inferPost ] U32.add_spec
+  [apply]     let* ⟨ y, y_post ⟩ ← [ +inferPost ] callFThenG_spec_step
+    case hf => let* ⟨ ⟩ ← [ +inferPost ] U32.add_spec_step
     case hg =>
       intros y a✝
-      let* ⟨ ⟩ ← [ +inferPost ] U32.add_spec
+      let* ⟨ ⟩ ← [ +inferPost ] U32.add_spec_step
     agrind
 -/
 #guard_msgs in
@@ -89,10 +89,10 @@ def callSlicemapM (x : Slice U32) : Result (Slice U32) := do
 /--
 info: Try this:
 
-  [apply]     let* ⟨ y, y_post1, y_post2 ⟩ ← [ +inferPost ] Slice.mapM_spec
+  [apply]     let* ⟨ y, y_post1, y_post2 ⟩ ← [ +inferPost ] Slice.mapM_spec_step
     case hf =>
       intros i hi
-      let* ⟨ ⟩ ← [ +inferPost ] U32.add_spec
+      let* ⟨ ⟩ ← [ +inferPost ] U32.add_spec_step
     agrind
 -/
 #guard_msgs in
@@ -112,14 +112,14 @@ def callSlicemapMTwice (x : Slice U32) : Result (Slice U32) := do
 /--
 info: Try this:
 
-  [apply]     let* ⟨ y, y_post1, y_post2 ⟩ ← [ +inferPost ] Slice.mapM_spec
+  [apply]     let* ⟨ y, y_post1, y_post2 ⟩ ← [ +inferPost ] Slice.mapM_spec_step
     case hf =>
       intros i hi
-      let* ⟨ ⟩ ← [ +inferPost ] U32.add_spec
-    let* ⟨ z, z_post1, z_post2 ⟩ ← [ +inferPost ] Slice.mapM_spec
+      let* ⟨ ⟩ ← [ +inferPost ] U32.add_spec_step
+    let* ⟨ z, z_post1, z_post2 ⟩ ← [ +inferPost ] Slice.mapM_spec_step
     case hf =>
       intros i hi
-      let* ⟨ ⟩ ← [ +inferPost ] U32.mul_spec
+      let* ⟨ ⟩ ← [ +inferPost ] U32.mul_spec_step
     agrind
 -/
 #guard_msgs in
